src/re.lean
@@ -40,25 +40,32 @@ pr_subset ha (by { simp, })
 lemma recuraive.k (A : set α) : k ∈ ℛ A := ⟨prec.k, ktot⟩
 lemma recuraive.s (A : set α) : s ∈ ℛ A := ⟨prec.s, stot⟩
 
-lemma prec.const (A : set α) {a : α} : a ∈ (ℰ A : set α) → 𝐤 a ∈ (ℰ A : set α) :=
+lemma prec.const {A : set α} {a : α} : a ∈ (ℰ A : set α) → 𝐤 a ∈ (ℰ A : set α) :=
 begin
   assume h : a ∈ ℰ A,
   have l0 : ↓k * ↓a = ↓𝐤 a, { simp, },
   show 𝐤 a ∈ ℰ A, from prec.mul l0 prec.k h,
 end
 
-lemma prec.subst (A : set α) {a b : α} :
+lemma prec.subst' {A : set α} {a : α} :
+  a ∈ ℰ A → 𝐬' a ∈ ℰ A :=
+begin
+  assume h : a ∈ ℰ A,
+  have l0 : ↓s * ↓a = ↓𝐬' a, { unfold subst', simp, },
+  show 𝐬' a ∈ ℰ A, from prec.mul l0 prec.s h,
+end
+
+lemma prec.subst {A : set α} {a b : α} :
   a ∈ ℰ A → b ∈ ℰ A → 𝐬 a b ∈ ℰ A :=
 begin
   assume (ha : a ∈ ℰ A) (hb : b ∈ ℰ A),
-  have l0 : ↓s * ↓a = ↓𝐬' a, { unfold subst', simp, },
-  have l1 : 𝐬' a ∈ (ℰ A : set α), from prec.mul l0 prec.s ha,
-  have l2 : ↓𝐬' a * ↓b = ↓𝐬 a b, { unfold subst', simp, },
-  show 𝐬 a b ∈ ℰ A, from prec.mul l2 l1 hb,
+  have l0 : 𝐬' a ∈ (ℰ A : set α), from prec.subst' ha,
+  have l1 : ↓𝐬' a * ↓b = ↓𝐬 a b, { unfold subst', simp, },
+  show 𝐬 a b ∈ ℰ A, from prec.mul l1 l0 hb,
 end
 
-lemma prec.i {A : set α} : i ∈ ℰ A := prec.subst A prec.k prec.k
-lemma recursive.i (A : set α) : i ∈ (ℛ A : set α) := ⟨prec.i, itot⟩
+@[simp] lemma prec.i {A : set α} : i ∈ ℰ A := prec.subst prec.k prec.k
+@[simp] lemma recursive.i (A : set α) : i ∈ (ℛ A : set α) := ⟨prec.i, itot⟩
 
 inductive lambda (A : set α) 
 | var : ℕ → lambda
@@ -101,14 +108,13 @@ notation n` →[`A`] `l := option.get (@lambda_defined _ _ A n l)
 notation n` →∅ `l := n →[∅] l
 notation n` →u `l := n →[set.univ] l
 
-
 lemma lambda_pr {A : set α} :
   ∀ {e : lambda A} (h : defined (expr A e) = tt), option.get h ∈ ℰ A
 | #_ _ := prec.k
 | &p _ := p
 | (l * m) h := begin
-    have ld : defined (expr A l) = tt, from defined_l h,
-    have md : defined (expr A m) = tt, from defined_r h,
+    have ld : defined (expr A l) = tt, from str_l h,
+    have md : defined (expr A m) = tt, from str_r h,
     have lpr : option.get ld ∈ ℰ A, from lambda_pr ld,
     have mpr : option.get md ∈ ℰ A, from lambda_pr md,
     have e : ↓option.get ld * ↓option.get md = ↓option.get h, { simp [expr], },
@@ -186,8 +192,39 @@ begin
     { exact ⟨fpr, fpr⟩, }, },
 end
 
+lemma nhbcdkjsvk (P Q : Prop) : ¬(P ∧ Q) → (¬P ∨ ¬Q) := by { exact not_and_distrib.mp}
+
+theorem total_ext [nontotal α] (A : set α) : ¬total_in (ℰ A) ∨ ¬extensional_in (ℰ A) :=
+begin
+  apply not_and_distrib.mp,
+  rintros ⟨h0 : total_in (ℰ A), h1 : extensional_in (ℰ A)⟩,
+  have e0 : (𝐬' k : α) = 𝐤 i,
+  { apply h1,
+    { show 𝐬' k ∈ ℰ A, from prec.subst' prec.k, },
+    { show 𝐤 i ∈ ℰ A, from prec.const prec.i, },
+    { intros x xpr,
+      simp,
+      apply h1,
+      { show 𝐬 k x ∈ ℰ A, from prec.subst prec.k xpr, },
+      { show i ∈ ℰ A, from prec.i, },
+      intros y ypr,
+      calc
+        ↓𝐬 k x * ↓y = ↓𝐤 y * ↓option.get (h0 xpr ypr) : by simp
+        ...         = ↓i * ↓y : by simp only [k_simp0, i_simp], }, },
+  have e1 : ↓(𝐤 div1 : α) * (↓div0 * ↓div1) = ↓div1,
+  { calc
+    ↓(𝐤 div1 : α) * (↓div0 * ↓div1) = ↓𝐬' k * ↓div0 * ↓div1 : by simp
+    ...                             = ↓𝐤 i * ↓div0 * ↓div1  : by rw e0
+    ...                             = ↓div1                 : by simp, },
+  have hd : defined (↓(𝐤 div1 : α) * (↓div0 * ↓div1)) = tt, { rw e1, refl, },
+  have c0 : defined (↓div0 * ↓div1 : option α) = tt, from str_r hd,
+  have c1 : defined (↓div0 * ↓div1 : option α) = ff, simp,
+  show false, from bool_iff_false.mpr c1 c0
+end
 
 end nontotal
+
+namespace reduciability
 
 def reducible (A : set α) (f g : α) : Prop := ∃ e : α, e ∈ ℰ A ∧ ↓e * ↓g = ↓f 
 def T_reducible (f g : α) : Prop := reducible ∅ f g
@@ -207,6 +244,8 @@ begin
   { show e_ac ∈ ℰ₀, simp, },
   { show ↓e_ac * ↓c = ↓a, simp [lam, expr, heab, hebc], },
 end
+
+end reduciability
 
 namespace jump
 /-
